clean up

code/bignum/Hacl.Impl.Exponentiation.fst
@@ -185,205 +185,6 @@ let lexp_pow2_in_place #a_t len ctx_len k ctx acc b =
     Loops.unfold_repeat (v b) k.to.concr_ops.SE.sqr (refl1 0) (v j);
     k.lsqr ctx acc acc)
 
-
-// Precomputed table [a^0 = one; a^1; a^2; ..; a^(table_len - 1)]
-//----------------------------------------------------------------
-
-inline_for_extraction noextract
-val lprecomp_table_mul:
-    #a_t:inttype_a
-  -> len:size_t{v len > 0}
-  -> ctx_len:size_t
-  -> k:concrete_ops a_t len ctx_len
-  -> ctx:lbuffer (uint_t a_t SEC) ctx_len
-  -> a:lbuffer (uint_t a_t SEC) len
-  -> i:size_t
-  -> ti:lbuffer (uint_t a_t SEC) len
-  -> res:lbuffer (uint_t a_t SEC) len ->
-  Stack unit
-  (requires fun h ->
-    live h a /\ live h ti /\ live h ctx /\ live h res /\
-    disjoint a ti /\ disjoint a ctx /\ disjoint a res /\
-    disjoint ti ctx /\ disjoint ti res /\ disjoint ctx res /\
-    k.to.linv (as_seq h a) /\ k.to.linv_ctx (as_seq h ctx) /\
-    k.to.linv (as_seq h ti) /\
-    k.to.refl (as_seq h ti) == SE.pow k.to.concr_ops (k.to.refl (as_seq h a)) (v i))
-  (ensures  fun h0 _ h1 -> modifies (loc res) h0 h1 /\
-    k.to.linv (as_seq h1 res) /\
-    k.to.refl (as_seq h1 res) == SE.pow k.to.concr_ops (k.to.refl (as_seq h0 a)) (v i + 1))
-
-let lprecomp_table_mul #a_t len ctx_len k ctx a i ti res =
-  let h0 = ST.get () in
-  k.lmul ctx a ti res;
-  let h1 = ST.get () in
-  assert (k.to.refl (as_seq h1 res) == k.to.concr_ops.SE.mul (k.to.refl (as_seq h0 a)) (k.to.refl (as_seq h0 ti)));
-  SE.pow_unfold k.to.concr_ops (k.to.refl (as_seq h0 a)) (v i + 1)
-
-
-#push-options "--z3rlimit 150"
-inline_for_extraction noextract
-val precomp_table_inv_lemma_j:
-    #a_t:inttype_a
-  -> len:size_t{v len > 0}
-  -> ctx_len:size_t
-  -> k:concrete_ops a_t len ctx_len
-  -> a:LSeq.lseq (uint_t a_t SEC) (v len)
-  -> table_len:size_t{v table_len * v len <= max_size_t}
-  -> table1:LSeq.lseq (uint_t a_t SEC) (v table_len * v len)
-  -> table2:LSeq.lseq (uint_t a_t SEC) (v table_len * v len)
-  -> i:nat{i <= v table_len}
-  -> j:nat{j < i} -> Lemma
-  (requires
-    LSeq.sub table1 0 (i * v len) == LSeq.sub table2 0 (i * v len) /\
-    precomp_table_inv len ctx_len k a table_len table1 j)
-  (ensures
-    precomp_table_inv len ctx_len k a table_len table2 j)
-
-let precomp_table_inv_lemma_j #a_t len ctx_len k a table_len table1 table2 i j =
-  assert (precomp_table_inv len ctx_len k a table_len table1 j);
-  Math.Lemmas.lemma_mult_le_right (v len) (j + 1) (v table_len);
-  let bj1 = LSeq.sub table1 (j * v len) (v len) in
-  let bj2 = LSeq.sub table2 (j * v len) (v len) in
-
-  let aux (l:nat{l < v len}) : Lemma (LSeq.index bj1 l == LSeq.index bj2 l) =
-    Seq.lemma_index_slice table1 (j * v len) (j * v len + v len) l;
-    assert (LSeq.index bj1 l == LSeq.index table1 (j * v len + l));
-    Seq.lemma_index_slice table2 (j * v len) (j * v len + v len) l;
-    assert (LSeq.index bj2 l == LSeq.index table2 (j * v len + l));
-    Seq.lemma_index_slice table1 0 (i * v len) (j * v len + l);
-    Seq.lemma_index_slice table2 0 (i * v len) (j * v len + l);
-    assert (LSeq.index table1 (j * v len + l) == LSeq.index table2 (j * v len + l));
-    assert (LSeq.index bj1 l == LSeq.index bj2 l) in
-
-  Classical.forall_intro aux;
-  LSeq.eq_intro bj1 bj2;
-  assert (precomp_table_inv len ctx_len k a table_len table2 j)
-#pop-options
-
-
-inline_for_extraction noextract
-val precomp_table_inv_lemma:
-    #a_t:inttype_a
-  -> len:size_t{v len > 0}
-  -> ctx_len:size_t
-  -> k:concrete_ops a_t len ctx_len
-  -> a:LSeq.lseq (uint_t a_t SEC) (v len)
-  -> table_len:size_t{v table_len * v len <= max_size_t}
-  -> table1:LSeq.lseq (uint_t a_t SEC) (v table_len * v len)
-  -> table2:LSeq.lseq (uint_t a_t SEC) (v table_len * v len)
-  -> i:nat{i <= v table_len} -> Lemma
-  (requires
-    LSeq.sub table1 0 (i * v len) == LSeq.sub table2 0 (i * v len) /\
-    (forall (j:nat{j < i}). precomp_table_inv len ctx_len k a table_len table1 j))
-  (ensures
-    (forall (j:nat{j < i}). precomp_table_inv len ctx_len k a table_len table2 j))
-
-let precomp_table_inv_lemma #a_t len ctx_len k a table_len table1 table2 i =
-  let aux (j:nat{j < i}) : Lemma (precomp_table_inv len ctx_len k a table_len table2 j) =
-    assert (precomp_table_inv len ctx_len k a table_len table1 j);
-    precomp_table_inv_lemma_j #a_t len ctx_len k a table_len table1 table2 i j;
-    assert (precomp_table_inv len ctx_len k a table_len table2 j) in
-
-  Classical.forall_intro aux
-
-
-inline_for_extraction noextract
-val lprecomp_table_f:
-    #a_t:inttype_a
-  -> len:size_t{v len > 0}
-  -> ctx_len:size_t
-  -> k:concrete_ops a_t len ctx_len
-  -> ctx:lbuffer (uint_t a_t SEC) ctx_len
-  -> a:lbuffer (uint_t a_t SEC) len
-  -> table_len:size_t{1 < v table_len /\ v table_len * v len <= max_size_t}
-  -> i:size_t{v i < v table_len - 1}
-  -> table:lbuffer (uint_t a_t SEC) (table_len *! len) ->
-  Stack unit
-  (requires fun h ->
-    live h a /\ live h table /\ live h ctx /\
-    disjoint a table /\ disjoint ctx table /\ disjoint a ctx /\
-    k.to.linv (as_seq h a) /\ k.to.linv_ctx (as_seq h ctx) /\
-    (forall (j:nat{j <= v i}).
-      precomp_table_inv len ctx_len k (as_seq h a) table_len (as_seq h table) j))
-  (ensures  fun h0 _ h1 -> modifies (loc table) h0 h1 /\
-    (forall (j:nat{j <= v i + 1}).
-      precomp_table_inv len ctx_len k (as_seq h0 a) table_len (as_seq h1 table) j))
-
-#push-options "--z3rlimit 300"
-let lprecomp_table_f #a_t len ctx_len k ctx a table_len i table =
-  Math.Lemmas.lemma_mult_le_right (v len) (v i + 1) (v table_len);
-  Math.Lemmas.lemma_mult_le_right (v len) (v i + 2) (v table_len);
-  assert (v (i *! len) == v i * v len);
-  assert (v (i *! len +! len) == v i * v len + v len);
-
-  let h0 = ST.get () in
-  assert (precomp_table_inv len ctx_len k (as_seq h0 a) table_len (as_seq h0 table) (v i));
-  let t1 = sub table (i *! len) len in
-  let t2 = sub table (i *! len +! len) len in
-  lprecomp_table_mul len ctx_len k ctx a i t1 t2;
-  let h1 = ST.get () in
-  B.modifies_buffer_elim (B.gsub #(uint_t a_t SEC) table 0ul (i *! len +! len)) (loc t2) h0 h1;
-  assert (precomp_table_inv len ctx_len k (as_seq h0 a) table_len (as_seq h1 table) (v i + 1));
-  LSeq.eq_intro
-    (LSeq.sub (as_seq h0 table) 0 (v i * v len + v len))
-    (LSeq.sub (as_seq h1 table) 0 (v i * v len + v len));
-
-  assert (forall (j:nat{j <= v i}).
-    precomp_table_inv len ctx_len k (as_seq h0 a) table_len (as_seq h0 table) j);
-  precomp_table_inv_lemma len ctx_len k (as_seq h0 a) table_len (as_seq h0 table) (as_seq h1 table) (v i + 1);
-  assert (forall (j:nat{j <= v i + 1}).
-    precomp_table_inv len ctx_len k (as_seq h0 a) table_len (as_seq h1 table) j)
-#pop-options
-
-
-let lprecomp_table #a_t len ctx_len k ctx a table_len table =
-  let t0 = sub table 0ul len in
-  let t1 = sub table len len in
-  k.lone ctx t0;
-  let h0 = ST.get () in
-  copy t1 a;
-  let h1 = ST.get () in
-  //B.modifies_buffer_elim (B.gsub #(uint_t a_t SEC) table 0ul len) (loc t1) h0 h1;
-  LSeq.eq_intro (as_seq h0 t0) (as_seq h1 t0);
-  assert (k.to.linv (as_seq h1 t0) /\ k.to.linv (as_seq h1 t1));
-  SE.pow_eq0 k.to.concr_ops (k.to.refl (as_seq h0 a));
-  assert (precomp_table_inv len ctx_len k (as_seq h0 a) table_len (as_seq h1 table) 0);
-
-  [@ inline_let]
-  let inv h (i:nat{i <= v table_len - 1}) =
-    modifies (loc table) h1 h /\
-    (forall (j:nat{j < i + 1}).
-      precomp_table_inv len ctx_len k (as_seq h a) table_len (as_seq h table) j) in
-
-
-  Lib.Loops.for 0ul (table_len -! 1ul) inv
-  (fun j ->
-    lprecomp_table_f #a_t len ctx_len k ctx a table_len j table)
-
-
-let lprecomp_get_vartime #a_t len ctx_len k l table_len ctx a table bits_l tmp =
-  let bits_l32 = Lib.RawIntTypes.(size_from_UInt32 (u32_to_UInt32 (to_u32 bits_l))) in
-  assert (v bits_l32 == v bits_l /\ v bits_l < v table_len);
-  Math.Lemmas.lemma_mult_le_right (v len) (v bits_l + 1) (v table_len);
-  assert (v (bits_l32 *! len) == v bits_l32 * v len);
-
-  let h0 = ST.get () in
-  let a_bits_l = sub table (bits_l32 *! len) len in
-  let h1 = ST.get () in
-  assert (precomp_table_inv len ctx_len k (as_seq h0 a) table_len (as_seq h0 table) (v bits_l));
-  assert (k.to.refl (as_seq h1 a_bits_l) == SE.pow k.to.concr_ops (k.to.refl (as_seq h0 a)) (v bits_l));
-  copy tmp a_bits_l
-
-
-let lprecomp_get_consttime #a_t len ctx_len k l table_len ctx a table bits_l tmp =
-  Math.Lemmas.lemma_mult_le_right (v len) (v bits_l + 1) (v table_len);
-  let h0 = ST.get () in
-  PT.table_select_consttime len table_len table bits_l tmp;
-  let h1 = ST.get () in
-  assert (as_seq h1 tmp == LSeq.sub (as_seq h0 table) (v bits_l * v len) (v len));
-  assert (precomp_table_inv len ctx_len k (as_seq h0 a) table_len (as_seq h0 table) (v bits_l));
-  assert (k.to.refl (as_seq h1 tmp) == SE.pow k.to.concr_ops (k.to.refl (as_seq h0 a)) (v bits_l))
-
 //---------------------------------------------------
 
 #set-options "--z3rlimit 100"
@@ -684,6 +485,70 @@ let mk_lexp_fw_table #a_t len ctx_len k l table_len table_inv pow_a_to_small_b c
 //-------------------------------------
 
 inline_for_extraction noextract
+let table_inv_precomp
+  (a_t:inttype_a)
+  (len:size_t{v len > 0})
+  (ctx_len:size_t)
+  (k:concrete_ops a_t len ctx_len)
+  (l:size_window_t a_t len)
+  (table_len:table_len_t len) : table_inv_t a_t len table_len =
+  fun a table ->
+    1 < v table_len /\ v table_len = pow2 (v l) /\
+      (forall (j:nat{j < v table_len}).
+      PT.precomp_table_inv len ctx_len k a table_len table j)
+
+
+// This function returns table.[bits_l] = a^bits_l
+// It takes variable time to access bits_l-th element of a table
+inline_for_extraction noextract
+val lprecomp_get_vartime:
+     #a_t:inttype_a
+  -> len:size_t{v len > 0}
+  -> ctx_len:size_t
+  -> k:concrete_ops a_t len ctx_len
+  -> l:size_window_t a_t len
+  -> table_len:table_len_t len ->
+  pow_a_to_small_b_st a_t len ctx_len k l table_len
+    (table_inv_precomp a_t len ctx_len k l table_len)
+
+let lprecomp_get_vartime #a_t len ctx_len k l table_len ctx a table bits_l tmp =
+  let bits_l32 = Lib.RawIntTypes.(size_from_UInt32 (u32_to_UInt32 (to_u32 bits_l))) in
+  assert (v bits_l32 == v bits_l /\ v bits_l < v table_len);
+  Math.Lemmas.lemma_mult_le_right (v len) (v bits_l + 1) (v table_len);
+  assert (v (bits_l32 *! len) == v bits_l32 * v len);
+
+  let h0 = ST.get () in
+  let a_bits_l = sub table (bits_l32 *! len) len in
+  let h1 = ST.get () in
+  assert (PT.precomp_table_inv len ctx_len k (as_seq h0 a) table_len (as_seq h0 table) (v bits_l));
+  assert (k.to.refl (as_seq h1 a_bits_l) == SE.pow k.to.concr_ops (k.to.refl (as_seq h0 a)) (v bits_l));
+  copy tmp a_bits_l
+
+
+// This function returns table.[bits_l] = a^bits_l
+// It takes constant time to access bits_l-th element of a table
+inline_for_extraction noextract
+val lprecomp_get_consttime:
+     #a_t:inttype_a
+  -> len:size_t{v len > 0}
+  -> ctx_len:size_t
+  -> k:concrete_ops a_t len ctx_len
+  -> l:size_window_t a_t len
+  -> table_len:table_len_t len ->
+  pow_a_to_small_b_st a_t len ctx_len k l table_len
+    (table_inv_precomp a_t len ctx_len k l table_len)
+
+let lprecomp_get_consttime #a_t len ctx_len k l table_len ctx a table bits_l tmp =
+  Math.Lemmas.lemma_mult_le_right (v len) (v bits_l + 1) (v table_len);
+  let h0 = ST.get () in
+  PT.table_select_consttime len table_len table bits_l tmp;
+  let h1 = ST.get () in
+  assert (as_seq h1 tmp == LSeq.sub (as_seq h0 table) (v bits_l * v len) (v len));
+  assert (PT.precomp_table_inv len ctx_len k (as_seq h0 a) table_len (as_seq h0 table) (v bits_l));
+  assert (k.to.refl (as_seq h1 tmp) == SE.pow k.to.concr_ops (k.to.refl (as_seq h0 a)) (v bits_l))
+
+
+inline_for_extraction noextract
 val lexp_fw_gen:
     #a_t:inttype_a
   -> len:size_t{v len > 0}
@@ -700,7 +565,7 @@ let lexp_fw_gen #a_t len ctx_len k l table_len lprecomp_get ctx a bLen bBits b r
   Math.Lemmas.pow2_lt_compat 32 (v l);
 
   let table = create (table_len *! len) (uint #a_t #SEC 0) in
-  lprecomp_table #a_t len ctx_len k ctx a table_len table;
+  PT.lprecomp_table #a_t len ctx_len k ctx a table_len table;
   let h = ST.get () in
 
   mk_lexp_fw_table len ctx_len k l table_len
