code/bignum/Hacl.Impl.Exponentiation.fsti
@@ -12,85 +12,11 @@ module LSeq = Lib.Sequence
 
 module SE = Spec.Exponentiation
 module BD = Hacl.Bignum.Definitions
+module PT = Hacl.Impl.PrecompTable
+
+include Hacl.Impl.Exponentiation.Definitions
 
 #reset-options "--z3rlimit 50 --fuel 0 --ifuel 0"
-
-inline_for_extraction noextract
-let inttype_a = t:inttype{t = U32 \/ t = U64}
-
-inline_for_extraction noextract
-class to_concrete_ops (a_t:inttype_a) (len:size_t{v len > 0}) (ctx_len:size_t) = {
-  t_spec: Type0;
-  concr_ops: SE.concrete_ops t_spec;
-  linv_ctx: x:LSeq.lseq (uint_t a_t SEC) (v ctx_len) -> Type0;
-  linv: x:LSeq.lseq (uint_t a_t SEC) (v len) -> Type0;
-  refl: x:LSeq.lseq (uint_t a_t SEC) (v len){linv x} -> GTot t_spec;
-}
-
-
-inline_for_extraction noextract
-let lone_st
-  (a_t:inttype_a)
-  (len:size_t{v len > 0})
-  (ctx_len:size_t)
-  (to:to_concrete_ops a_t len ctx_len) =
-    ctx:lbuffer (uint_t a_t SEC) ctx_len
-  -> x:lbuffer (uint_t a_t SEC) len ->
-  Stack unit
-  (requires fun h ->
-    live h x /\ live h ctx /\ disjoint ctx x /\
-    to.linv_ctx (as_seq h ctx))
-  (ensures  fun h0 _ h1 -> modifies (loc x) h0 h1 /\
-    to.linv (as_seq h1 x) /\
-    to.refl (as_seq h1 x) == to.concr_ops.SE.one ())
-
-
-inline_for_extraction noextract
-let lmul_st
-  (a_t:inttype_a)
-  (len:size_t{v len > 0})
-  (ctx_len:size_t)
-  (to:to_concrete_ops a_t len ctx_len) =
-    ctx:lbuffer (uint_t a_t SEC) ctx_len
-  -> x:lbuffer (uint_t a_t SEC) len
-  -> y:lbuffer (uint_t a_t SEC) len
-  -> xy:lbuffer (uint_t a_t SEC) len ->
-  Stack unit
-  (requires fun h ->
-    live h x /\ live h y /\ live h xy /\ live h ctx /\
-    eq_or_disjoint x xy /\ eq_or_disjoint y xy /\ eq_or_disjoint x y /\
-    disjoint ctx x /\ disjoint ctx y /\ disjoint ctx xy /\
-    to.linv (as_seq h x) /\ to.linv (as_seq h y) /\ to.linv_ctx (as_seq h ctx))
-  (ensures fun h0 _ h1 -> modifies (loc xy) h0 h1 /\ to.linv (as_seq h1 xy) /\
-    to.refl (as_seq h1 xy) == to.concr_ops.SE.mul (to.refl (as_seq h0 x)) (to.refl (as_seq h0 y)))
-
-
-inline_for_extraction noextract
-let lsqr_st
-  (a_t:inttype_a)
-  (len:size_t{v len > 0})
-  (ctx_len:size_t)
-  (to:to_concrete_ops a_t len ctx_len) =
-    ctx:lbuffer (uint_t a_t SEC) ctx_len
-  -> x:lbuffer (uint_t a_t SEC) len
-  -> xx:lbuffer (uint_t a_t SEC) len ->
-  Stack unit
-  (requires fun h ->
-    live h x /\ live h xx /\ live h ctx /\
-    disjoint x ctx /\ disjoint xx ctx /\ eq_or_disjoint x xx /\
-    to.linv (as_seq h x) /\ to.linv_ctx (as_seq h ctx))
-  (ensures fun h0 _ h1 -> modifies (loc xx) h0 h1 /\ to.linv (as_seq h1 xx) /\
-    to.refl (as_seq h1 xx) == to.concr_ops.SE.sqr (refl (as_seq h0 x)))
-
-
-inline_for_extraction noextract
-class concrete_ops (a_t:inttype_a) (len:size_t{v len > 0}) (ctx_len:size_t) = {
-  to: Ghost.erased (to_concrete_ops a_t len ctx_len);
-  lone: lone_st a_t len ctx_len to;
-  lmul: lmul_st a_t len ctx_len to;
-  lsqr: lsqr_st a_t len ctx_len to;
-}
-
 
 // This function computes `a^b` using a binary right-to-left method
 // It takes variable time to compute the result
@@ -186,47 +112,8 @@ val lexp_pow2_in_place:
     k.to.refl (as_seq h1 a) == SE.exp_pow2 k.to.concr_ops (k.to.refl (as_seq h0 a)) (v b))
 
 
-// Precomputed table [a^0 = one; a^1; a^2; ..; a^(table_len - 1)]
-//----------------------------------------------------------------
-
-inline_for_extraction noextract
-let precomp_table_inv
-  (#a_t:inttype_a)
-  (len:size_t{v len > 0})
-  (ctx_len:size_t)
-  (k:concrete_ops a_t len ctx_len)
-  (a:LSeq.lseq (uint_t a_t SEC) (v len))
-  (table_len:size_t{v table_len * v len <= max_size_t})
-  (table:LSeq.lseq (uint_t a_t SEC) (v table_len * v len))
-  (j:nat{j < v table_len}) : Type0
- =
-  Math.Lemmas.lemma_mult_le_right (v len) (j + 1) (v table_len);
-  let bj = LSeq.sub table (j * v len) (v len) in
-  k.to.linv bj /\ k.to.linv a /\
-  k.to.refl bj == SE.pow k.to.concr_ops (k.to.refl a) j
-
-
-// This function computes [a^0 = one; a^1; a^2; ..; a^(table_len - 1)]
-inline_for_extraction noextract
-val lprecomp_table:
-    #a_t:inttype_a
-  -> len:size_t{v len > 0}
-  -> ctx_len:size_t
-  -> k:concrete_ops a_t len ctx_len
-  -> ctx:lbuffer (uint_t a_t SEC) ctx_len
-  -> a:lbuffer (uint_t a_t SEC) len
-  -> table_len:size_t{1 < v table_len /\ v table_len * v len <= max_size_t}
-  -> table:lbuffer (uint_t a_t SEC) (table_len *! len) ->
-  Stack unit
-  (requires fun h ->
-    live h a /\ live h table /\ live h ctx /\
-    disjoint a table /\ disjoint ctx table /\ disjoint a ctx /\
-    k.to.linv (as_seq h a) /\ k.to.linv_ctx (as_seq h ctx))
-  (ensures  fun h0 _ h1 -> modifies (loc table) h0 h1 /\
-    (forall (j:nat{j < v table_len}).{:pattern precomp_table_inv len ctx_len k (as_seq h1 a) table_len (as_seq h1 table) j}
-      precomp_table_inv len ctx_len k (as_seq h1 a) table_len (as_seq h1 table) j))
-
-//-----------------------------------------
+// Fixed-window method using a precomputed table
+//----------------------------------------------
 
 inline_for_extraction noextract
 let size_window_t (a_t:inttype_a) (len:size_t{v len > 0}) =
@@ -239,7 +126,7 @@ let table_len_t (len:size_t{v len > 0}) =
 inline_for_extraction noextract
 let table_inv_t (a_t:inttype_a) (len:size_t{v len > 0}) (table_len:table_len_t len) =
   a:LSeq.lseq (uint_t a_t SEC) (v len)
-    -> table:LSeq.lseq (uint_t a_t SEC) (v (table_len *! len)) -> GTot Type0
+  -> table:LSeq.lseq (uint_t a_t SEC) (v (table_len *! len)) -> GTot Type0
 
 
 inline_for_extraction noextract
@@ -267,49 +154,6 @@ let pow_a_to_small_b_st
     k.to.linv (as_seq h1 res) /\
     k.to.refl (as_seq h1 res) == SE.pow k.to.concr_ops (k.to.refl (as_seq h0 a)) (v b))
 
-
-inline_for_extraction noextract
-let table_inv_precomp
-  (a_t:inttype_a)
-  (len:size_t{v len > 0})
-  (ctx_len:size_t)
-  (k:concrete_ops a_t len ctx_len)
-  (l:size_window_t a_t len)
-  (table_len:table_len_t len) : table_inv_t a_t len table_len =
-  fun a table ->
-    1 < v table_len /\ v table_len = pow2 (v l) /\
-      (forall (j:nat{j < v table_len}).
-      precomp_table_inv len ctx_len k a table_len table j)
-
-
-// This function returns table.[bits_l] = a^bits_l
-// It takes variable time to access bits_l-th element of a table
-inline_for_extraction noextract
-val lprecomp_get_vartime:
-     #a_t:inttype_a
-  -> len:size_t{v len > 0}
-  -> ctx_len:size_t
-  -> k:concrete_ops a_t len ctx_len
-  -> l:size_window_t a_t len
-  -> table_len:table_len_t len ->
-  pow_a_to_small_b_st a_t len ctx_len k l table_len
-    (table_inv_precomp a_t len ctx_len k l table_len)
-
-
-// This function returns table.[bits_l] = a^bits_l
-// It takes constant time to access bits_l-th element of a table
-inline_for_extraction noextract
-val lprecomp_get_consttime:
-     #a_t:inttype_a
-  -> len:size_t{v len > 0}
-  -> ctx_len:size_t
-  -> k:concrete_ops a_t len ctx_len
-  -> l:size_window_t a_t len
-  -> table_len:table_len_t len ->
-  pow_a_to_small_b_st a_t len ctx_len k l table_len
-    (table_inv_precomp a_t len ctx_len k l table_len)
-
-//-----------------------------
 
 inline_for_extraction noextract
 let lexp_fw_table_st
