code/bignum/Hacl.Impl.PrecompTable.fst
@@ -10,19 +10,21 @@ open Lib.IntTypes
 open Lib.Buffer
 
 module ST = FStar.HyperStack.ST
+module B = LowStar.Buffer
+
 module LSeq = Lib.Sequence
 module Loops = Lib.LoopCombinators
 
 module BB = Hacl.Bignum.Base
+module BD = Hacl.Bignum.Definitions
 module PT = Hacl.Spec.PrecompTable
-
-open Hacl.Spec.Bignum.Definitions
+module SE = Spec.Exponentiation
 
 #reset-options "--z3rlimit 50 --fuel 0 --ifuel 0"
 
 inline_for_extraction noextract
 val table_select_consttime_f:
-    #t:limb_t
+    #t:BD.limb_t
   -> len:size_t{v len > 0}
   -> table_len:size_t{1 < v table_len /\ v table_len * v len <= max_size_t}
   -> table:lbuffer (uint_t t SEC) (table_len *! len)
@@ -44,21 +46,6 @@ let table_select_consttime_f #t len table_len table i j acc =
   let res_j = sub table ((j +! 1ul) *! len) len in
   map2T len acc (BB.mask_select c) res_j acc
 
-
-inline_for_extraction noextract
-val table_select_consttime:
-    #t:limb_t
-  -> len:size_t{v len > 0}
-  -> table_len:size_t{1 < v table_len /\ v table_len * v len <= max_size_t}
-  -> table:lbuffer (uint_t t SEC) (table_len *! len)
-  -> i:uint_t t SEC{v i < v table_len}
-  -> res:lbuffer (uint_t t SEC) len ->
-  Stack unit
-  (requires fun h ->
-    (v i + 1) * v len <= v table_len * v len /\
-    live h table /\ live h res /\ disjoint table res)
-  (ensures  fun h0 _ h1 -> modifies (loc res) h0 h1 /\
-    as_seq h1 res == LSeq.sub (as_seq h0 table) (v i * v len) (v len))
 
 let table_select_consttime #t len table_len table i res =
   let h0 = ST.get () in
@@ -82,3 +69,177 @@ let table_select_consttime #t len table_len table i res =
       (PT.table_select_f (v len) (v table_len) (as_seq h0 table) i) (as_seq h1 res) (v j);
     table_select_consttime_f len table_len table i j res);
   PT.table_select_lemma (v len) (v table_len) (as_seq h0 table) i
+
+// Precomputed table [a^0 = one; a^1; a^2; ..; a^(table_len - 1)]
+//----------------------------------------------------------------
+
+inline_for_extraction noextract
+val lprecomp_table_mul:
+    #a_t:inttype_a
+  -> len:size_t{v len > 0}
+  -> ctx_len:size_t
+  -> k:concrete_ops a_t len ctx_len
+  -> ctx:lbuffer (uint_t a_t SEC) ctx_len
+  -> a:lbuffer (uint_t a_t SEC) len
+  -> i:size_t
+  -> ti:lbuffer (uint_t a_t SEC) len
+  -> res:lbuffer (uint_t a_t SEC) len ->
+  Stack unit
+  (requires fun h ->
+    live h a /\ live h ti /\ live h ctx /\ live h res /\
+    disjoint a ti /\ disjoint a ctx /\ disjoint a res /\
+    disjoint ti ctx /\ disjoint ti res /\ disjoint ctx res /\
+    k.to.linv (as_seq h a) /\ k.to.linv_ctx (as_seq h ctx) /\
+    k.to.linv (as_seq h ti) /\
+    k.to.refl (as_seq h ti) == SE.pow k.to.concr_ops (k.to.refl (as_seq h a)) (v i))
+  (ensures  fun h0 _ h1 -> modifies (loc res) h0 h1 /\
+    k.to.linv (as_seq h1 res) /\
+    k.to.refl (as_seq h1 res) == SE.pow k.to.concr_ops (k.to.refl (as_seq h0 a)) (v i + 1))
+
+let lprecomp_table_mul #a_t len ctx_len k ctx a i ti res =
+  let h0 = ST.get () in
+  k.lmul ctx a ti res;
+  let h1 = ST.get () in
+  assert (k.to.refl (as_seq h1 res) == k.to.concr_ops.SE.mul (k.to.refl (as_seq h0 a)) (k.to.refl (as_seq h0 ti)));
+  SE.pow_unfold k.to.concr_ops (k.to.refl (as_seq h0 a)) (v i + 1)
+
+
+#push-options "--z3rlimit 150"
+inline_for_extraction noextract
+val precomp_table_inv_lemma_j:
+    #a_t:inttype_a
+  -> len:size_t{v len > 0}
+  -> ctx_len:size_t
+  -> k:concrete_ops a_t len ctx_len
+  -> a:LSeq.lseq (uint_t a_t SEC) (v len)
+  -> table_len:size_t{v table_len * v len <= max_size_t}
+  -> table1:LSeq.lseq (uint_t a_t SEC) (v table_len * v len)
+  -> table2:LSeq.lseq (uint_t a_t SEC) (v table_len * v len)
+  -> i:nat{i <= v table_len}
+  -> j:nat{j < i} -> Lemma
+  (requires
+    LSeq.sub table1 0 (i * v len) == LSeq.sub table2 0 (i * v len) /\
+    precomp_table_inv len ctx_len k a table_len table1 j)
+  (ensures
+    precomp_table_inv len ctx_len k a table_len table2 j)
+
+let precomp_table_inv_lemma_j #a_t len ctx_len k a table_len table1 table2 i j =
+  assert (precomp_table_inv len ctx_len k a table_len table1 j);
+  Math.Lemmas.lemma_mult_le_right (v len) (j + 1) (v table_len);
+  let bj1 = LSeq.sub table1 (j * v len) (v len) in
+  let bj2 = LSeq.sub table2 (j * v len) (v len) in
+
+  let aux (l:nat{l < v len}) : Lemma (LSeq.index bj1 l == LSeq.index bj2 l) =
+    Seq.lemma_index_slice table1 (j * v len) (j * v len + v len) l;
+    assert (LSeq.index bj1 l == LSeq.index table1 (j * v len + l));
+    Seq.lemma_index_slice table2 (j * v len) (j * v len + v len) l;
+    assert (LSeq.index bj2 l == LSeq.index table2 (j * v len + l));
+    Seq.lemma_index_slice table1 0 (i * v len) (j * v len + l);
+    Seq.lemma_index_slice table2 0 (i * v len) (j * v len + l);
+    assert (LSeq.index table1 (j * v len + l) == LSeq.index table2 (j * v len + l));
+    assert (LSeq.index bj1 l == LSeq.index bj2 l) in
+
+  Classical.forall_intro aux;
+  LSeq.eq_intro bj1 bj2;
+  assert (precomp_table_inv len ctx_len k a table_len table2 j)
+#pop-options
+
+
+inline_for_extraction noextract
+val precomp_table_inv_lemma:
+    #a_t:inttype_a
+  -> len:size_t{v len > 0}
+  -> ctx_len:size_t
+  -> k:concrete_ops a_t len ctx_len
+  -> a:LSeq.lseq (uint_t a_t SEC) (v len)
+  -> table_len:size_t{v table_len * v len <= max_size_t}
+  -> table1:LSeq.lseq (uint_t a_t SEC) (v table_len * v len)
+  -> table2:LSeq.lseq (uint_t a_t SEC) (v table_len * v len)
+  -> i:nat{i <= v table_len} -> Lemma
+  (requires
+    LSeq.sub table1 0 (i * v len) == LSeq.sub table2 0 (i * v len) /\
+    (forall (j:nat{j < i}). precomp_table_inv len ctx_len k a table_len table1 j))
+  (ensures
+    (forall (j:nat{j < i}). precomp_table_inv len ctx_len k a table_len table2 j))
+
+let precomp_table_inv_lemma #a_t len ctx_len k a table_len table1 table2 i =
+  let aux (j:nat{j < i}) : Lemma (precomp_table_inv len ctx_len k a table_len table2 j) =
+    assert (precomp_table_inv len ctx_len k a table_len table1 j);
+    precomp_table_inv_lemma_j #a_t len ctx_len k a table_len table1 table2 i j;
+    assert (precomp_table_inv len ctx_len k a table_len table2 j) in
+
+  Classical.forall_intro aux
+
+
+inline_for_extraction noextract
+val lprecomp_table_f:
+    #a_t:inttype_a
+  -> len:size_t{v len > 0}
+  -> ctx_len:size_t
+  -> k:concrete_ops a_t len ctx_len
+  -> ctx:lbuffer (uint_t a_t SEC) ctx_len
+  -> a:lbuffer (uint_t a_t SEC) len
+  -> table_len:size_t{1 < v table_len /\ v table_len * v len <= max_size_t}
+  -> i:size_t{v i < v table_len - 1}
+  -> table:lbuffer (uint_t a_t SEC) (table_len *! len) ->
+  Stack unit
+  (requires fun h ->
+    live h a /\ live h table /\ live h ctx /\
+    disjoint a table /\ disjoint ctx table /\ disjoint a ctx /\
+    k.to.linv (as_seq h a) /\ k.to.linv_ctx (as_seq h ctx) /\
+    (forall (j:nat{j <= v i}).
+      precomp_table_inv len ctx_len k (as_seq h a) table_len (as_seq h table) j))
+  (ensures  fun h0 _ h1 -> modifies (loc table) h0 h1 /\
+    (forall (j:nat{j <= v i + 1}).
+      precomp_table_inv len ctx_len k (as_seq h0 a) table_len (as_seq h1 table) j))
+
+#push-options "--z3rlimit 300"
+let lprecomp_table_f #a_t len ctx_len k ctx a table_len i table =
+  Math.Lemmas.lemma_mult_le_right (v len) (v i + 1) (v table_len);
+  Math.Lemmas.lemma_mult_le_right (v len) (v i + 2) (v table_len);
+  assert (v (i *! len) == v i * v len);
+  assert (v (i *! len +! len) == v i * v len + v len);
+
+  let h0 = ST.get () in
+  assert (precomp_table_inv len ctx_len k (as_seq h0 a) table_len (as_seq h0 table) (v i));
+  let t1 = sub table (i *! len) len in
+  let t2 = sub table (i *! len +! len) len in
+  lprecomp_table_mul len ctx_len k ctx a i t1 t2;
+  let h1 = ST.get () in
+  B.modifies_buffer_elim (B.gsub #(uint_t a_t SEC) table 0ul (i *! len +! len)) (loc t2) h0 h1;
+  assert (precomp_table_inv len ctx_len k (as_seq h0 a) table_len (as_seq h1 table) (v i + 1));
+  LSeq.eq_intro
+    (LSeq.sub (as_seq h0 table) 0 (v i * v len + v len))
+    (LSeq.sub (as_seq h1 table) 0 (v i * v len + v len));
+
+  assert (forall (j:nat{j <= v i}).
+    precomp_table_inv len ctx_len k (as_seq h0 a) table_len (as_seq h0 table) j);
+  precomp_table_inv_lemma len ctx_len k (as_seq h0 a) table_len (as_seq h0 table) (as_seq h1 table) (v i + 1);
+  assert (forall (j:nat{j <= v i + 1}).
+    precomp_table_inv len ctx_len k (as_seq h0 a) table_len (as_seq h1 table) j)
+#pop-options
+
+
+let lprecomp_table #a_t len ctx_len k ctx a table_len table =
+  let t0 = sub table 0ul len in
+  let t1 = sub table len len in
+  k.lone ctx t0;
+  let h0 = ST.get () in
+  copy t1 a;
+  let h1 = ST.get () in
+  //B.modifies_buffer_elim (B.gsub #(uint_t a_t SEC) table 0ul len) (loc t1) h0 h1;
+  LSeq.eq_intro (as_seq h0 t0) (as_seq h1 t0);
+  assert (k.to.linv (as_seq h1 t0) /\ k.to.linv (as_seq h1 t1));
+  SE.pow_eq0 k.to.concr_ops (k.to.refl (as_seq h0 a));
+  assert (precomp_table_inv len ctx_len k (as_seq h0 a) table_len (as_seq h1 table) 0);
+
+  [@ inline_let]
+  let inv h (i:nat{i <= v table_len - 1}) =
+    modifies (loc table) h1 h /\
+    (forall (j:nat{j < i + 1}).
+      precomp_table_inv len ctx_len k (as_seq h a) table_len (as_seq h table) j) in
+
+
+  Lib.Loops.for 0ul (table_len -! 1ul) inv
+  (fun j ->
+    lprecomp_table_f #a_t len ctx_len k ctx a table_len j table)
