code/bignum/Hacl.Impl.Exponentiation.Definitions.fst
@@ -1,0 +1,90 @@
+module Hacl.Impl.Exponentiation.Definitions
+
+open FStar.HyperStack
+open FStar.HyperStack.ST
+open FStar.Mul
+
+open Lib.IntTypes
+open Lib.Buffer
+
+module ST = FStar.HyperStack.ST
+module LSeq = Lib.Sequence
+module SE = Spec.Exponentiation
+
+#reset-options "--z3rlimit 50 --fuel 0 --ifuel 0"
+
+inline_for_extraction noextract
+let inttype_a = t:inttype{t = U32 \/ t = U64}
+
+inline_for_extraction noextract
+class to_concrete_ops (a_t:inttype_a) (len:size_t{v len > 0}) (ctx_len:size_t) = {
+  t_spec: Type0;
+  concr_ops: SE.concrete_ops t_spec;
+  linv_ctx: x:LSeq.lseq (uint_t a_t SEC) (v ctx_len) -> Type0;
+  linv: x:LSeq.lseq (uint_t a_t SEC) (v len) -> Type0;
+  refl: x:LSeq.lseq (uint_t a_t SEC) (v len){linv x} -> GTot t_spec;
+}
+
+
+inline_for_extraction noextract
+let lone_st
+  (a_t:inttype_a)
+  (len:size_t{v len > 0})
+  (ctx_len:size_t)
+  (to:to_concrete_ops a_t len ctx_len) =
+    ctx:lbuffer (uint_t a_t SEC) ctx_len
+  -> x:lbuffer (uint_t a_t SEC) len ->
+  Stack unit
+  (requires fun h ->
+    live h x /\ live h ctx /\ disjoint ctx x /\
+    to.linv_ctx (as_seq h ctx))
+  (ensures  fun h0 _ h1 -> modifies (loc x) h0 h1 /\
+    to.linv (as_seq h1 x) /\
+    to.refl (as_seq h1 x) == to.concr_ops.SE.one ())
+
+
+inline_for_extraction noextract
+let lmul_st
+  (a_t:inttype_a)
+  (len:size_t{v len > 0})
+  (ctx_len:size_t)
+  (to:to_concrete_ops a_t len ctx_len) =
+    ctx:lbuffer (uint_t a_t SEC) ctx_len
+  -> x:lbuffer (uint_t a_t SEC) len
+  -> y:lbuffer (uint_t a_t SEC) len
+  -> xy:lbuffer (uint_t a_t SEC) len ->
+  Stack unit
+  (requires fun h ->
+    live h x /\ live h y /\ live h xy /\ live h ctx /\
+    eq_or_disjoint x xy /\ eq_or_disjoint y xy /\ eq_or_disjoint x y /\
+    disjoint ctx x /\ disjoint ctx y /\ disjoint ctx xy /\
+    to.linv (as_seq h x) /\ to.linv (as_seq h y) /\ to.linv_ctx (as_seq h ctx))
+  (ensures fun h0 _ h1 -> modifies (loc xy) h0 h1 /\ to.linv (as_seq h1 xy) /\
+    to.refl (as_seq h1 xy) == to.concr_ops.SE.mul (to.refl (as_seq h0 x)) (to.refl (as_seq h0 y)))
+
+
+inline_for_extraction noextract
+let lsqr_st
+  (a_t:inttype_a)
+  (len:size_t{v len > 0})
+  (ctx_len:size_t)
+  (to:to_concrete_ops a_t len ctx_len) =
+    ctx:lbuffer (uint_t a_t SEC) ctx_len
+  -> x:lbuffer (uint_t a_t SEC) len
+  -> xx:lbuffer (uint_t a_t SEC) len ->
+  Stack unit
+  (requires fun h ->
+    live h x /\ live h xx /\ live h ctx /\
+    disjoint x ctx /\ disjoint xx ctx /\ eq_or_disjoint x xx /\
+    to.linv (as_seq h x) /\ to.linv_ctx (as_seq h ctx))
+  (ensures fun h0 _ h1 -> modifies (loc xx) h0 h1 /\ to.linv (as_seq h1 xx) /\
+    to.refl (as_seq h1 xx) == to.concr_ops.SE.sqr (refl (as_seq h0 x)))
+
+
+inline_for_extraction noextract
+class concrete_ops (a_t:inttype_a) (len:size_t{v len > 0}) (ctx_len:size_t) = {
+  to: Ghost.erased (to_concrete_ops a_t len ctx_len);
+  lone: lone_st a_t len ctx_len to;
+  lmul: lmul_st a_t len ctx_len to;
+  lsqr: lsqr_st a_t len ctx_len to;
+}
