code/bignum/Hacl.Impl.PrecompTable.fsti
@@ -1,0 +1,76 @@
+module Hacl.Impl.PrecompTable
+
+open FStar.Mul
+
+open FStar.HyperStack
+open FStar.HyperStack.ST
+open FStar.Mul
+
+open Lib.IntTypes
+open Lib.Buffer
+
+module ST = FStar.HyperStack.ST
+module LSeq = Lib.Sequence
+
+module SE = Spec.Exponentiation
+module BD = Hacl.Bignum.Definitions
+
+include Hacl.Impl.Exponentiation.Definitions
+
+#reset-options "--z3rlimit 50 --fuel 0 --ifuel 0"
+
+inline_for_extraction noextract
+val table_select_consttime:
+    #t:BD.limb_t
+  -> len:size_t{v len > 0}
+  -> table_len:size_t{1 < v table_len /\ v table_len * v len <= max_size_t}
+  -> table:lbuffer (uint_t t SEC) (table_len *! len)
+  -> i:uint_t t SEC{v i < v table_len}
+  -> res:lbuffer (uint_t t SEC) len ->
+  Stack unit
+  (requires fun h ->
+    (v i + 1) * v len <= v table_len * v len /\
+    live h table /\ live h res /\ disjoint table res)
+  (ensures  fun h0 _ h1 -> modifies (loc res) h0 h1 /\
+    as_seq h1 res == LSeq.sub (as_seq h0 table) (v i * v len) (v len))
+
+
+// Precomputed table [a^0 = one; a^1; a^2; ..; a^(table_len - 1)]
+//----------------------------------------------------------------
+
+inline_for_extraction noextract
+let precomp_table_inv
+  (#a_t:inttype_a)
+  (len:size_t{v len > 0})
+  (ctx_len:size_t)
+  (k:concrete_ops a_t len ctx_len)
+  (a:LSeq.lseq (uint_t a_t SEC) (v len))
+  (table_len:size_t{v table_len * v len <= max_size_t})
+  (table:LSeq.lseq (uint_t a_t SEC) (v table_len * v len))
+  (j:nat{j < v table_len}) : Type0
+ =
+  Math.Lemmas.lemma_mult_le_right (v len) (j + 1) (v table_len);
+  let bj = LSeq.sub table (j * v len) (v len) in
+  k.to.linv bj /\ k.to.linv a /\
+  k.to.refl bj == SE.pow k.to.concr_ops (k.to.refl a) j
+
+
+// This function computes [a^0 = one; a^1; a^2; ..; a^(table_len - 1)]
+inline_for_extraction noextract
+val lprecomp_table:
+    #a_t:inttype_a
+  -> len:size_t{v len > 0}
+  -> ctx_len:size_t
+  -> k:concrete_ops a_t len ctx_len
+  -> ctx:lbuffer (uint_t a_t SEC) ctx_len
+  -> a:lbuffer (uint_t a_t SEC) len
+  -> table_len:size_t{1 < v table_len /\ v table_len * v len <= max_size_t}
+  -> table:lbuffer (uint_t a_t SEC) (table_len *! len) ->
+  Stack unit
+  (requires fun h ->
+    live h a /\ live h table /\ live h ctx /\
+    disjoint a table /\ disjoint ctx table /\ disjoint a ctx /\
+    k.to.linv (as_seq h a) /\ k.to.linv_ctx (as_seq h ctx))
+  (ensures  fun h0 _ h1 -> modifies (loc table) h0 h1 /\
+    (forall (j:nat{j < v table_len}).{:pattern precomp_table_inv len ctx_len k (as_seq h1 a) table_len (as_seq h1 table) j}
+      precomp_table_inv len ctx_len k (as_seq h1 a) table_len (as_seq h1 table) j))
